getter filtering of false positives ... however, there seems to be something fishy in InfeasibleReport.java

gravy/src/org/gravy/report/InfeasibleReport.java
@@ -3,6 +3,7 @@
  */
 package org.gravy.report;
 
+import java.util.HashMap;
 import java.util.HashSet;
 import java.util.LinkedList;
 import java.util.Set;
@@ -33,7 +34,9 @@ public class InfeasibleReport extends Report {
 			AbstractTransitionRelation tr, Set<BasicBlock> feasibleBlocks,
 			Set<BasicBlock> infeasibleBlocks) {
 		this.procedureName = tr.getProcedureName();
-		infeasibleSubProgs = findInfeasibleSubprogs(cff, infeasibleBlocks);
+		//infeasibleSubProgs = findInfeasibleSubprogs(cff, infeasibleBlocks);
+		infeasibleSubProgs = findInfeasibleSubGraphs(cff, infeasibleBlocks);
+		
 	}
 	
 	
@@ -85,6 +88,144 @@ public class InfeasibleReport extends Report {
 		return res;
 	}
 	
+	
+
+	private LinkedList<HashSet<Statement>> findInfeasibleSubGraphs(AbstractControlFlowFactory cff, Set<BasicBlock> infeasibleBlocks) {
+		LinkedList<HashSet<Statement>> res = new LinkedList<HashSet<Statement>>();
+		LinkedList<BasicBlock> allblocks = new LinkedList<BasicBlock>();
+		allblocks.addAll(infeasibleBlocks);
+		while (!allblocks.isEmpty()) {
+			HashSet<BasicBlock> subprog = new HashSet<BasicBlock>();
+			LinkedList<BasicBlock> todo = new LinkedList<BasicBlock>();
+			todo.add(allblocks.pop());
+			while (!todo.isEmpty()) {
+				BasicBlock current = todo.pop();
+				allblocks.remove(current);
+				subprog.add(current);
+				
+				for (BasicBlock b : current.getPredecessors()) {
+					if (!subprog.contains(b) && !todo.contains(b) && allblocks.contains(b)) {
+						todo.add(b);
+					}
+				}
+				for (BasicBlock b : current.getSuccessors()) {
+					if (!subprog.contains(b) && !todo.contains(b) && allblocks.contains(b)) {
+						todo.add(b);
+					}
+				}	
+			}		
+			
+			//now compute the source and the sinks of the subgraph.
+			//note, that there can only be one source
+			//but several sinks.
+			BasicBlock source=null;
+			HashSet<BasicBlock> sinks=new HashSet<BasicBlock>();
+			for (BasicBlock b : subprog) {
+				boolean connected = false;
+				for (BasicBlock x : b.getPredecessors()) {
+					if (subprog.contains(x)) {
+						connected = true; break;
+					}
+				}
+				if (!connected) {
+					if (source!=null) System.err.println("ups");
+					source = b;
+				}
+				connected = false;
+				for (BasicBlock x : b.getSuccessors()) {
+					if (subprog.contains(x)) {
+						connected = true; break;
+					}
+				}
+				if (!connected) {					
+					sinks.add(b);
+				}				
+			}
+			
+			
+			HashSet<Statement> stmts = computeCleanedStmtList(cff, subprog, source, sinks);
+			if (stmts.size()>0) {				
+				res.add(stmts);
+			}
+		}
+		return res;
+	}
+	
+	private HashSet<Statement> computeCleanedStmtList(AbstractControlFlowFactory cff, HashSet<BasicBlock> subgraph, BasicBlock source, HashSet<BasicBlock> sinks) {
+		if (subgraph.size()==0 || source==null || sinks.size()==0) {
+			return new HashSet<Statement>(); 
+		}
+		//the following code finds all blocks that must
+		//be reached on every paths from source to sink.
+		//I.e., it works it BFSs from the sink and keeps the set
+		//of visited Blocks and intersects them at joins.
+		LinkedList<BasicBlock> todo = new LinkedList<BasicBlock>();
+		HashSet<BasicBlock> done = new HashSet<BasicBlock>();
+		HashMap<BasicBlock, HashSet<BasicBlock>> mustReach = new HashMap<BasicBlock, HashSet<BasicBlock>>();
+		todo.addAll(sinks);
+		while (!todo.isEmpty()) {
+			BasicBlock current = todo.removeLast();
+			//check if all predecessors have been processed already.
+			//if not, add the block to the end of the cue and start over
+			boolean allGood = true;
+			for (BasicBlock prev : current.getSuccessors()) {
+				if (!subgraph.contains(prev)) continue;
+				if (!done.contains(prev)) {
+					allGood=false;
+					break;
+				}
+			}		
+			if (!allGood){
+				todo.addFirst(current);
+				continue;
+			}
+			//if all predecessors have been processed,
+			//we can compute the dominators list by
+			//intersecting the list of all predecessors
+			HashSet<BasicBlock> currentDom = null;
+			if (!sinks.contains(current)) {
+				for (BasicBlock prev : current.getSuccessors()) {
+					if (!subgraph.contains(prev)) continue;
+					if (currentDom == null) {
+						currentDom = new HashSet<BasicBlock>(mustReach.get(prev));
+					} else {
+						//retainAll computes the intersection of the two sets.
+						currentDom.retainAll(mustReach.get(prev));
+					}				
+				}		
+			}
+			//special case, only occurs for the root/sink
+			if (currentDom == null) {
+				currentDom = new HashSet<BasicBlock>();
+			}
+			currentDom.add(current); //of course, a block dominates itself
+			mustReach.put(current, currentDom);
+			done.add(current);	
+			for (BasicBlock next : current.getPredecessors()) {
+				if (!todo.contains(next) && !done.contains(next)) {
+					if (!subgraph.contains(next)) continue;
+					todo.addLast(next);
+				}
+			}			
+		}	
+		
+		HashSet<Statement> ret = new HashSet<Statement>();
+		for (BasicBlock b : subgraph) {			
+			if (this.containsNamedAttribute(b, ProgramFactory.Cloned)) {
+				if (mustReach.get(source).contains(b)) {
+					//in that case, drop the entire report
+					//because any path contains a cloned statement
+					return new HashSet<Statement>();
+				}
+			} else {
+				for (CfgStatement stmt : b.getStatements()) {
+					Statement s = cff.findAstStatement(stmt);
+					if (s!=null) ret.add(s);
+				}
+			}
+		}
+		return ret;
+	}
 	
 	
 	@Override 
